tests/NerodiaTests/basic.lean
@@ -15,8 +15,41 @@ open Nerodia
 /-- info: some "hello"  -/
 #guard_msgs in
 #eval PyIO.toIO do
-  let bytes ← (← mkPyStr "hello").utf8Encode
+  let bytes ← (← mkPyStr "hello").encodeUTF8
   return String.fromUTF8? bytes.toByteArray
+
+/--
+info: 3
+3
+[119, 111, 119]
+wow
+-/
+#guard_msgs in
+#eval do
+  let bytes ← PyIO.toIO do
+    mkPyBytes (.mk #[119, 111, 119])
+  IO.println bytes.size
+  IO.println bytes.usize
+  IO.println bytes.toByteArray
+  let str ← PyIO.toIO do
+    bytes.decodeUTF8
+  IO.println str
+
+/-- info: [237, 160, 128] -/
+#guard_msgs in
+#eval PyIO.toIO do
+  let bytes ← mkPyBytes (.mk #[0xED, 0xA0, 0x80])
+  let str ← bytes.decode .utf8 .surrogatePass
+  let roundtrip ← str.encode .utf8 .surrogatePass
+  return roundtrip.toByteArray
+
+/-- info: "�" -/
+#guard_msgs in
+#eval PyIO.toIO do
+  let bytes ← mkPyBytes (.mk #[0xED, 0xA0, 0x80])
+  let str ← bytes.decode .utf8 .surrogatePass
+  -- Test that `toString` handles lone surrogates
+  return str.toString
 
 /-- info: "None" -/
 #guard_msgs in
